Lean 4 version of automatic-complexity-of-list-repeat.lean

automatic-complexity-of-list-repeat.lean
@@ -1,8 +1,6 @@
-import computability.DFA computability.NFA
-import data.fintype.basic
-import data.fintype.fin
+import Mathlib.Computability.DFA
 
-open list
+open List
 /-
 In this file we quite simply prove that the automatic complexity of a "repeat" word like
 000000000
@@ -22,137 +20,193 @@ theorem complexity_of_repeat
     TwoState_step
 
 -/
-constant u:ℕ
-def α := {l : ℕ // l < u} -- The input alphabet
-
-def σ := fin 2 -- The set of states
+-- open Classical
 
 
-def q0 := (⟨0,zero_lt_two⟩:σ)
-def q1 := (⟨1, one_lt_two⟩:σ)
+axiom u:ℕ
+def α := Fin u --{l : ℕ // l < u} -- The input alphabet
 
-def TwoState (z:α) : DFA α σ := -- the two-state DFA that accepts z^n
+-- def (Fin 2) := Fin 2 -- The set of states
+
+noncomputable instance : DecidableEq α := by exact Classical.decEq α
+noncomputable instance : DecidableEq (Fin 2) := by exact Classical.decEq (Fin 2)
+
+def q0 := (⟨0, Nat.succ_pos 1⟩:(Fin 2))
+def q1 := (⟨1, Nat.one_lt_succ_succ 0⟩:(Fin 2))
+
+
+noncomputable def TwoState (z:α) : DFA α (Fin 2) := -- the two-state DFA that accepts z^n
   DFA.mk
-    (λ q, λ b : α, -- transition ("step") function
+    (λ q ↦ λ b : α ↦ -- transition ("step") function
     ite (q=q0) (ite (b=z) q0 q1) q1)
     q0             -- start state
     {q0}           -- set of accept states
     
-def uniquely_accepts {τ: Type} (M: DFA α τ) (s: list α) :=
-    ∀ t : list α,
+def uniquely_accepts {τ: Type} (M: DFA α τ) (s: List α) :=
+    ∀ t : List α,
       t.length = s.length  →
          (M.accepts t ↔ t=s)
 
 
-def automatic_complexity_is_at_most : list α → ℕ → Prop := λ s, λ k,
+def automatic_complexity_is_at_most : List α → ℕ → Prop := λ s k ↦
 -- this should be: ∃ k' ≤ k, because *intentionally* it is not guaranteed that the set of cardinalities
 -- for which a uniquely accepting DFA exists is closed upward.
-  ∃ M : DFA α (fin k), -- the set of states is a prefix and subtype of ℕ
+  ∃ M : DFA α (Fin k), -- the set of states is a prefix and subtype of ℕ
   uniquely_accepts M s
 
 
 theorem q0_ne_q1: q0 ≠ q1 :=
-  λ he, zero_ne_one (congr_arg (λ x:σ, x.1) he)
+  λ he ↦ zero_ne_one (congr_arg (λ x:(Fin 2) ↦ x.1) he)
 
 theorem TwoState_stay_q0 {a z:α} (h: (TwoState z).eval [a] = q0) : a = z :=
-  let M := (TwoState z) in
-  have a ≠ z → M.eval [a] ≠ q0, from
-    λ h,
-      have hw: M.eval [a] = q1, from
-        calc M.step q0 a = (ite (true) (ite (a = z) q0 q1) q1): rfl
-                     ... = q1: by {cc,},
-      have q0 ≠ q1, from q0_ne_q1,
-      by cc,
-  by cc
+  let M := (TwoState z)
+  have : a ≠ z → (TwoState z).eval [a] ≠ q0 :=
+    λ h ↦
+      have hw: (TwoState z).eval [a] = q1 :=
+        calc
+        (TwoState z).step q0 a = (ite (true) (ite (a = z) q0 q1) q1)  := eq_ite_iff.mpr (by {
+          left
+          constructor
+          rfl
+          unfold TwoState
+          exact if_pos rfl
+        })
+        _ = q1                                     := by {
+        have : (if true = true then if a = z then q0 else q1 else q1)
+             = (if a = z then q0 else q1)
+        := rfl
+        rw [this]
+        exact if_neg h
+        }
+      have : q0 ≠ q1 := q0_ne_q1
+      by {
+        intro hcontra
+        rw [hw] at hcontra
+        exact this hcontra.symm
+      }
+  by {
+    by_contra H
+    exact this H h
+  }
 
-theorem TwoState_stay_q1 (z:α) (x:list α): (TwoState z).eval_from q1 x = q1 :=
-  list.rec_on x rfl (λ _ _ h, h) -- kind of surprised this works
+
+theorem TwoState_stay_q1 (z:α) (x:List α): (TwoState z).evalFrom q1 x = q1 :=
+  List.recOn x rfl (λ a y h ↦ by {
+    have t3 : q1 ≠ q0 := q0_ne_q1.symm
+    have t2 : DFA.evalFrom (TwoState z) q1 [a] = q1 := by {
+      have t1: DFA.evalFrom (TwoState z) q1 [a] =
+      DFA.step (TwoState z) q1 a :=
+        DFA.evalFrom_singleton _ _ _
+      rw [t1]
+      exact if_neg t3      
+    }
+    have t1 : DFA.evalFrom (TwoState z) q1 (a :: y) =
+    DFA.evalFrom (TwoState z) (DFA.evalFrom (TwoState z) q1 [a]) y := rfl
+    rw [t2] at t1
+    rw [h] at t1
+    exact t1
+  }) -- kind of surprised this works
 
 
-theorem TwoState_accepts_repeat {z :α} {n : ℕ} : (TwoState z).eval (repeat z n) = q0:=
+theorem TwoState_accepts_repeat {z :α} {n : ℕ} : (TwoState z).eval (List.replicate n z) = q0:=
 
-  let M := (TwoState z) in
-  have TwoState_step: M.step M.start z = q0, from
-    calc M.step M.start z = ite (M.start = q0) (ite (z = z) q0 q1)  q1: rfl
-                      ... = ite (M.start = q0) (q0)                 q1: by cc,
-  nat.rec_on n (rfl) (λ n h, calc
-      _ = foldl M.step (M.step M.start z) (repeat z n) : rfl
-    ... = foldl M.step q0                 (repeat z n) : by rw TwoState_step
-    ... = q0: h
+  let M := (TwoState z)
+  have TwoState_step: M.step M.start z = q0 :=
+    (
+    calc
+    M.step M.start z = ite (M.start = q0) (ite (z = z) q0 q1)  q1 := rfl
+    _ = ite (M.start = q0) (q0)                                q1 := by {
+      exact congr_arg (λ q ↦ if M.start = q0 then q else q1) (if_pos rfl)
+    }
+    _ = q0 := by exact if_pos rfl
+    )
+  Nat.recOn n (rfl) (λ n h ↦ calc
+  _ = foldl M.step (M.step M.start z) (List.replicate n z) := rfl
+  _ = foldl M.step q0                 (List.replicate n z) := by rw [TwoState_step]
+  _ = q0 := h
   )
 
 
 
 
-lemma either_or {a : σ}  (h : a.1≠ 1) : a.1=0 :=
-  iff.elim_left nat.lt_one_iff (array.push_back_idx a.2 h)
+theorem either_or {a : (Fin 2)}  (h : a.1≠ 1) : a.1=0 := by {
+  have : a.1 < 2 := a.2
+  have : a.1 ≤ 1 := by exact Fin.is_le a
+  have : a.1 < 1 := by exact Nat.lt_of_le_of_ne this h
+  exact Nat.lt_one_iff.mp this
+}
 
-lemma either_or_strong {a : σ} (not_zero : a ≠ q0) : a = q1 :=
-  have h1: a.1 = 1, from by_contra (
-    λ not_one, not_zero (fin.eq_of_veq (either_or not_one))
-  ),
-  fin.eq_of_veq h1
 
-theorem TwoState_no_return_to_q0 {q:σ} {z:α}{x:list α}
-  (h:(TwoState z).eval_from q x = q0): q=q0 :=
+  --Iff.elim_left Nat.lt_one_iff (array.push_back_idx a.2 h)
+
+theorem either_or_strong {a : (Fin 2)} (not_zero : a ≠ q0) : a = q1 :=
+  have h1: a.1 = 1 := by_contra (
+    λ not_one ↦ not_zero (Fin.eq_of_veq (either_or not_one))
+  )
+  Fin.eq_of_veq h1
+
+theorem TwoState_no_return_to_q0 {q:(Fin 2)} {z:α}{x:List α}
+  (h:(TwoState z).evalFrom q x = q0): q=q0 :=
   by_contra (
-    λ hh: q ≠ q0,
-    have h1: q = q1, from either_or_strong hh,
+    λ hh: q ≠ q0 ↦
+    have h1: q = q1 := either_or_strong hh
 
-    have h01: q0 = q1, from calc
-              q0 = (TwoState z).eval_from q  x : h.symm
-             ... = (TwoState z).eval_from q1 x : congr_arg (λ r, (TwoState z).eval_from r x) h1
-             ... = q1                          : TwoState_stay_q1 z x,
+    have h01: q0 = q1 := calc
+              q0 = (TwoState z).evalFrom q  x := h.symm
+             _ = (TwoState z).evalFrom q1 x   := congr_arg (λ r ↦ (TwoState z).evalFrom r x) h1
+             _ = q1                           := TwoState_stay_q1 z x
     q0_ne_q1 h01
   )
 
-theorem TwoState_accepts_only_starts_z {a z:α} {y:list α}
+theorem TwoState_accepts_only_starts_z {a z:α} {y:List α}
   (hq0:(TwoState z).eval (a :: y) = q0): a = z :=
   TwoState_stay_q0 (
     by_contra (
-      λ h,
-      let M := (TwoState z) in
-      have h1: M.step q0 a = q1, from either_or_strong h,
-      have hq1: M.eval (a :: y) = q1, from
-        calc M.eval_from (M.step q0 a) y
-          = M.eval_from q1 y : by rw h1
-      ... = q1               : TwoState_stay_q1 z y,
+      λ h ↦
+      let M := (TwoState z)
+      have h1: M.step q0 a = q1 := either_or_strong h
+      have hq1: M.eval (a :: y) = q1 :=
+        calc M.evalFrom (M.step q0 a) y
+        = M.evalFrom q1 y := by rw [h1]
+        _ = q1                := TwoState_stay_q1 z y
 
-      (ne_of_eq_of_ne hq1 (ne.symm q0_ne_q1)) hq0
+      (ne_of_eq_of_ne hq1 (Ne.symm q0_ne_q1)) hq0
     )
   )
 
-theorem TwoState_accepts_only_repeat {z :α} {x:list α}:
-(TwoState z).eval x = q0 → x = repeat z x.length := -- proof long because a::x defined "backwards"
-list.rec_on x (λ h, rfl) (
-    λ a x h_ind hq0,
-    let M := (TwoState z) in
-    have h0 : M.step q0 a = q0, from TwoState_no_return_to_q0 hq0,
+theorem TwoState_accepts_only_repeat {z :α} {x:List α}:
+(TwoState z).eval x = q0 → x = List.replicate x.length z := -- proof long because a::x deFined "backwards"
+List.recOn x (λ h ↦ rfl) (
+    λ a x h_ind hq0 ↦
+    let M := (TwoState z)
+    have h0 : M.step q0 a = q0 := TwoState_no_return_to_q0 hq0
 
-    have can_ind: M.eval x = q0, from
-      by_contra (λ hh: M.eval x ≠ q0,
-        have q0 = q1, from
-          calc q0 = M.eval_from (M.step q0 a) x : hq0.symm
-              ... = M.eval_from q0 x            : congr_arg (λ u, M.eval_from u x) h0
-              ... = q1                          : either_or_strong hh,
+    have can_ind: M.eval x = q0 :=
+      by_contra (λ hh: M.eval x ≠ q0 ↦
+        have : q0 = q1 :=
+          calc q0 = M.evalFrom (M.step q0 a) x := hq0.symm
+              _ = M.evalFrom q0 x              := congr_arg (λ u ↦ M.evalFrom u x) h0
+              _ = q1                           := either_or_strong hh
         q0_ne_q1 this
-      ),
+      )
 
-    calc _ = a :: (repeat z x.length): congr_arg _ (h_ind can_ind)
-       ... = z :: (repeat z x.length): congr_arg _ (TwoState_accepts_only_starts_z hq0)
+    calc _ = a :: (List.replicate x.length z) := congr_arg _ (h_ind can_ind)
+    _ = z :: (List.replicate x.length z)   := congr_arg (
+      λ b ↦ b :: replicate (length x) z
+    ) (TwoState_accepts_only_starts_z hq0)
 )
 
-theorem complexity_of_repeat (z:α) (n:ℕ): automatic_complexity_is_at_most (repeat z n) 2 :=
-  let M := (TwoState z) in
-  have n2: M.accepts (repeat z n), from TwoState_accepts_repeat,
-  exists.intro M (λ t h,
-    have mp: M.accepts t → t=(repeat z n), from
-      λ ha,
-      calc t = repeat z t.length            : TwoState_accepts_only_repeat ha
-         ... = repeat z (repeat z n).length : by rw h
-         ... = repeat z n                   : by rw (length_repeat z n),
+theorem complexity_of_repeat (z:α) (n:ℕ): automatic_complexity_is_at_most (List.replicate n z) 2 :=
+  let M := (TwoState z)
+  have n2: M.accepts (List.replicate n z) := TwoState_accepts_repeat
+  Exists.intro M (λ t h ↦
+    have mp: M.accepts t → t=(List.replicate n z) :=
+      λ ha ↦
+      calc t = List.replicate t.length z            := TwoState_accepts_only_repeat ha
+      _ = List.replicate (List.replicate n z).length z := by rw [h]
+      _ = List.replicate n z                   := by rw [List.length_replicate n z]
 
-    have mpr: t=(repeat z n) → M.accepts t, from λ his, by {rw ← his at n2,exact n2,},
+    have mpr: t=(List.replicate n z) → M.accepts t := λ his ↦ by {rw [← his] at n2;exact n2}
 
-    iff.intro mp mpr
+    Iff.intro mp mpr
   )
